finished proof of initialize and the overall structure of enqueue. Similar cases must be handeled, and impossible cases must be discarded. Some clean up is also required.

theories/twoLockMSQ.v
@@ -1,3 +1,4 @@
+From stdpp Require Import countable.
 From iris.algebra Require Import excl.
 From iris.heap_lang Require Import lang proofmode notation.
 From iris.heap_lang.lib Require Import lock spin_lock.
@@ -89,14 +90,14 @@ Context `{!inG Σ (exclR unitO)}.
 
 Let N := nroot .@ "twoLockMSQ".
 
-Record Qgnames := {γ_Hlock : gname;
-				  γ_Tlock : gname;
-				  γ_E : gname;
-				  γ_nE : gname;
-				  γ_D : gname;
-				  γ_nD : gname;
-				  γ_Before : gname;
-				  γ_After : gname;
+Record Qgnames := {γ_Hlock 	: gname;
+				   γ_Tlock 	: gname;
+				   γ_E 		: gname;
+				   γ_nE 	: gname;
+				   γ_D 		: gname;
+				   γ_nD 	: gname;
+				   γ_Before : gname;
+				   γ_After 	: gname;
 				  }.
 
 Definition TokHlock (g : Qgnames) := own g.(γ_Hlock) (Excl ()).
@@ -110,26 +111,127 @@ Definition TokAfter (g : Qgnames) := own g.(γ_After) (Excl ()).
 Definition TokUpdated (g : Qgnames) := ((TokBefore g) ∗ (TokAfter g))%I.
 
 (* Notaion for triples *)
-Notation fst x := (let '(a, b, c) := x in a).
-Notation snd x := (let '(a, b, c) := x in b).
-Notation trd x := (let '(a, b, c) := x in c).
+Definition fst {A B C} (x : A * B * C ) := (let '(a, b, c) := x in a).
+Definition snd {A B C} (x : A * B * C ) := (let '(a, b, c) := x in b).
+Definition trd {A B C} (x : A * B * C ) := (let '(a, b, c) := x in c).
 
 
 Fixpoint isLL_chain (xs : list (loc * val * loc) ) : iProp Σ :=
 	match xs with
 	| [] => True
-	| [(l'₁, v₁, l₂)] => l'₁ ↦□ (v₁, #l₂)
-	| (l'ᵢ₁, vᵢ₁, lᵢ₂) :: (((l'ᵢ, vᵢ, lᵢ₁) :: xs'') as xs') =>
-		l'ᵢ₁ ↦□ (vᵢ₁, #lᵢ₂) ∗
-		lᵢ₁ ↦□ #l'ᵢ₁ ∗ isLL_chain xs'
+	| [x] => (fst x) ↦□ (snd x, #(trd x))
+	| xᵢ₁ :: ((xᵢ :: xs'') as xs') =>
+		fst(xᵢ₁) ↦□ (snd xᵢ₁, #(trd xᵢ₁)) ∗
+		(trd xᵢ) ↦□ #(fst xᵢ₁) ∗ isLL_chain xs'
 	end.
+
+(* TODO: Prove this! *)
+Global Instance isLL_chain_persistent xs : Persistent (isLL_chain xs).
+Proof.
+	Admitted.
 
 Definition isLL (xs : list (loc * val * loc) ) : iProp Σ :=
 	match xs with
 	| [] => True
-	| (l'ₙ, vₙ, lₙ₁) :: xs' => lₙ₁ ↦ NONEV ∗ isLL_chain xs
+	| x :: xs' => (trd x) ↦ NONEV ∗ isLL_chain xs
 	end.
 
+Lemma isLL_and_chain : forall xs,
+	isLL xs -∗
+	isLL xs ∗ isLL_chain xs.
+Proof.
+	iIntros (xs) "HisLLxs".
+	destruct xs as [| x' xs']; first done.
+	unfold isLL.
+	iPoseProof "HisLLxs" as "[Htrdx' #HisLLxs]".
+	auto.
+Qed.
+
+Lemma fst_equal (x y : (loc * val * loc)) :
+	⌜#(fst x) = #(fst y)⌝ -∗
+	fst x ↦□ (snd x, #(trd x)) -∗
+	fst y ↦□ (snd y, #(trd y)) -∗
+	⌜x = y⌝.
+Proof.
+	iIntros (Heq_loc) "Hx Hy".
+	simplify_eq.
+	rewrite Heq_loc.
+	iCombine "Hx Hy" gives "[_ %Heq_pair]".
+	simplify_eq.
+	iPureIntro.
+	destruct x as [[lx1 vx] lx2], y as [[ly1 vy] ly2].
+	cbn in *.
+	by subst.
+Qed.
+
+Lemma isLL_chain_node : forall xs_1 x xs_2,
+	isLL_chain (xs_1 ++ x :: xs_2) -∗
+	fst(x) ↦□ (snd x, #(trd x)).
+Proof.
+	iIntros (xs_1 x xs_2) "#HisLL_chain".
+	iInduction xs_1 as [| y xs'_1] "IH".
+	- simpl.
+	  destruct xs_2.
+	  + done.
+	  + iDestruct "HisLL_chain" as "(Hx & _ & _)"; auto.
+	- iApply "IH". destruct xs'_1 as [| y' xs''_1];
+	  	iDestruct "HisLL_chain" as "(_ & _ & H)"; done.
+Qed.
+
+Lemma isLL_chain_split : forall xs ys,
+	isLL_chain (xs ++ ys) -∗
+	isLL_chain xs ∗ isLL_chain ys.
+Proof.
+	iIntros (xs ys) "#HisLL_chain_xs_ys".
+	iInduction xs as [|x' xs'] "IH".
+	- auto.
+	- destruct xs' as [| x'' xs''].
+	  + destruct ys as [| y' ys'].
+		* auto.
+		* iDestruct "HisLL_chain_xs_ys" as "(Hx' & Htrdy' & HIsLL_chain_ys')".
+		  fold isLL_chain. iSplitL; done.
+	  + iAssert (isLL_chain (x'' :: xs'') ∗ isLL_chain ys)%I as "[IHxs' IHys]".
+	  	{
+			iApply "IH". iDestruct "HisLL_chain_xs_ys" as "(_ & _ & Hchain)"; done.
+		}
+		iSplitL; auto.
+		iDestruct "HisLL_chain_xs_ys" as "(Hfstx' & Htrdx'' & _)".
+		unfold isLL_chain; auto.
+Qed.
+
+Lemma isLL_chain_agree : forall x_1 y_1 xs ys,
+	⌜fst x_1 = fst y_1⌝ -∗
+	isLL_chain (xs ++ [x_1]) -∗
+	isLL_chain (ys ++ [y_1]) -∗
+	⌜x_1 = y_1⌝.
+Proof.
+	iIntros (x_1 y_1 xs ys Heqfst_x1y1) "#HisLL_chainxs #HisLL_chainys".
+	iApply fst_equal.
+	- iPureIntro. by rewrite Heqfst_x1y1.
+	- by iApply (isLL_chain_node xs x_1 []).
+	- by iApply (isLL_chain_node ys y_1 []).
+Qed.
+
+Lemma isLL_chain_agree_next : forall x y z ys zs,
+	isLL_chain (ys ++ [y ; x]) -∗
+	isLL_chain (zs ++ [z ; x]) -∗
+	⌜y = z⌝.
+Proof.
+	iIntros (x y z ys zs) "#HisLL_chainys #HisLL_chainzs".
+	iAssert (isLL_chain ys ∗ isLL_chain ([y ; x]))%I as "[_ HisLL_chainy]".
+	{ by iApply isLL_chain_split. }
+	iAssert (isLL_chain zs ∗ isLL_chain ([z ; x]))%I as "[_ HisLL_chainz]".
+	{ by iApply isLL_chain_split. }
+	unfold isLL_chain.
+	iDestruct "HisLL_chainy" as "(#Hfsty_2 & #Htrdy_1 & Hfsty_1)".
+	iDestruct "HisLL_chainz" as "(#Hfsztz_2 & #Htrdz_1 & Hfstz_1)".
+	iCombine "Htrdy_1 Htrdz_1" gives "[_ %Heq_fst]".
+	simplify_eq.
+	iApply fst_equal; auto. iPureIntro. by rewrite Heq_fst.
+Qed.
+
+
+(* Todo: consider removing *)
 Lemma isLL_extend : forall xs (x y : (loc * val * loc)),
 	{{{ isLL (x :: xs) ∗
 		fst y ↦□ (snd y, #(trd y)) ∗
@@ -137,7 +239,7 @@ Lemma isLL_extend : forall xs (x y : (loc * val * loc)),
 			#(trd x) <- #(fst y)
 	{{{ w, RET w; isLL (y :: x :: xs) }}}.
 Proof.
-	iIntros (xs ((l'ₙ, vₙ), lₙ₁) ((l'ₙ₁, vₙ₁), lₙ₂) Φ) "([Hlₙ₁ HisLL_chain_xs] & Hfsty & Htrdy) HΦ".
+	iIntros (xs x y Φ) "([Hlₙ₁ HisLL_chain_xs] & Hfsty & Htrdy) HΦ".
 	wp_store.
 	iMod (pointsto_persist with "Hlₙ₁") as "Hlₙ₁".
 	iApply "HΦ".
@@ -147,22 +249,22 @@ Qed.
 Definition isLast {A} (x : A) xs := ∃ xs_rest, xs = x :: xs_rest.
 Definition isSndLast {A} (x : A) xs := ∃ x_first xs_rest, xs = x_first :: x :: xs_rest.
 
-Definition queue_invariant (head tail : loc) (Q_γ : Qgnames) : iProp Σ :=
+Definition queue_invariant (l_head l_tail : loc) (Q_γ : Qgnames) : iProp Σ :=
 	∃ xs xs_rest xs_old (x_head x_tail: (loc * val * loc)),
 	⌜xs = xs_rest ++ [x_head] ++ xs_old⌝ ∗
 	isLL xs ∗
 	(
 		(* Static *)
 		(
-			head ↦ #(fst x_head) ∗
-			tail ↦ #(fst x_tail) ∗ ⌜isLast x_tail xs⌝ ∗
+			l_head ↦ #(fst x_head) ∗
+			l_tail ↦ #(fst x_tail) ∗ ⌜isLast x_tail xs⌝ ∗
 			ToknE Q_γ ∗ ToknD Q_γ ∗ TokUpdated Q_γ
 		)
 		∨
 		(* Enqueue *)
 		(
-			head ↦ #(fst x_head) ∗
-			tail ↦{#1/2} #(fst x_tail) ∗
+			l_head ↦ #(fst x_head) ∗
+			l_tail ↦{#1/2} #(fst x_tail) ∗
 				(⌜isLast x_tail xs⌝ ∗ TokBefore Q_γ ∨
 				 ⌜isSndLast x_tail xs⌝ ∗ TokAfter Q_γ) ∗
 			TokE Q_γ ∗ ToknD Q_γ
@@ -170,15 +272,15 @@ Definition queue_invariant (head tail : loc) (Q_γ : Qgnames) : iProp Σ :=
 		∨
 		(* Dequeue *)
 		(
-			head ↦{#1/2} #(fst x_head) ∗
-			tail ↦ #(fst x_tail) ∗ ⌜isLast x_tail xs⌝ ∗
+			l_head ↦{#1/2} #(fst x_head) ∗
+			l_tail ↦ #(fst x_tail) ∗ ⌜isLast x_tail xs⌝ ∗
 			ToknE Q_γ ∗ TokD Q_γ ∗ TokUpdated Q_γ
 		)
 		∨
 		(* Both *)
 		(
-			head ↦{#1/2} #(fst x_head) ∗
-			tail ↦{#1/2} #(fst x_tail) ∗
+			l_head ↦{#1/2} #(fst x_head) ∗
+			l_tail ↦{#1/2} #(fst x_tail) ∗
 				(⌜isLast x_tail xs⌝ ∗ TokBefore Q_γ ∨
 				 ⌜isSndLast x_tail xs⌝ ∗ TokAfter Q_γ) ∗
 			TokE Q_γ ∗ TokD Q_γ
@@ -193,117 +295,208 @@ Definition is_queue (q : val) (Q_γ: Qgnames) : iProp Σ :=
 		is_lock Q_γ.(γ_Hlock) H_lock (TokD Q_γ) ∗
 		is_lock Q_γ.(γ_Tlock) T_lock (TokE Q_γ).
 
-(* TODO: Finish proof. *)
 Lemma initialize_spec : {{{ True }}} 
 							initialize #() 
 						{{{ v Q_γ, RET v; is_queue v Q_γ}}}.
 Proof.
 	iIntros (Φ) "_ HΦ".
-	wp_lam. 
+	wp_lam.
 	wp_pures.
+	wp_alloc l_2 as "Hl_2".
+	wp_alloc l'_1 as "Hl'_1".
+	wp_pures.
+	iMod (pointsto_persist with "Hl'_1") as "#Hl'_1".
+	wp_pures.
+	iMod (own_alloc (Excl ()) ) as (γ_D) "Hγ_D"; first done.
+	wp_apply (newlock_spec with "Hγ_D").
+	iIntros (hlock γ_Hlock) "Hγ_Hlock".
+	wp_let.
 	iMod (own_alloc (Excl ()) ) as (γ_E) "Hγ_E"; first done.
-	wp_alloc null' as "Hnull'".
-	iMod (pointsto_persist with "Hnull'") as "#Hnull'".
-	wp_alloc null as "Hnull".
-	wp_pures.
-	wp_alloc node' as "Hnode'".
-	iMod (pointsto_persist with "Hnode'") as "#Hnode'".
-	wp_pures.
-	wp_alloc head as "Hhead".
+	wp_apply (newlock_spec with "Hγ_E").
+	iIntros (tlock γ_Tlock) "Hγ_Tlock".
 	wp_let.
-	iMod (inv_alloc N _ (∃x xs, node_inv node' (x :: xs)) with "[Hnull]") as "#HnodeInv".
+	wp_alloc l_tail as "Hl_tail".
+	wp_alloc l_head as "Hl_head".
+	iMod (own_alloc (Excl ()) ) as (γ_nE) "Hγ_nE"; first done.
+	iMod (own_alloc (Excl ()) ) as (γ_nD) "Hγ_nD"; first done.
+	iMod (own_alloc (Excl ()) ) as (γ_Before) "Hγ_Before"; first done.
+	iMod (own_alloc (Excl ()) ) as (γ_After) "Hγ_After"; first done.
+	set (Queue_gnames := {| γ_Hlock := γ_Hlock;
+							γ_Tlock := γ_Tlock;
+							γ_E := γ_E;
+							γ_nE := γ_nE;
+							γ_D := γ_D;
+							γ_nD := γ_nD;
+							γ_Before := γ_Before;
+							γ_After := γ_After
+					|}).
+	iMod (inv_alloc N _ (queue_invariant l_head l_tail Queue_gnames) with "[Hl_head Hl_tail Hl'_1 Hl_2 Hγ_nE Hγ_nD Hγ_Before Hγ_After]") as "#HqueueInv".
 	{
-		iNext. iExists NONEV, []. cbn. iExists null. auto.
+		iNext. iExists [(l'_1, NONEV, l_2)], [], [], (l'_1, NONEV, l_2), (l'_1, NONEV, l_2). cbn. iSplitR; first done. iSplitL "Hl'_1 Hl_2"; first auto.
+		iLeft. iFrame. iPureIntro. exists []. reflexivity.
 	}
-	iAssert (head_prop head)%I with "[Hhead]" as "Hhead_prop".
-	{
-		iExists node'. auto.
-	}
-	wp_alloc tail as "Htail".
-	wp_let.
-	iAssert (head_prop tail)%I with "[Htail]" as "Htail_prop".
-	{
-		iExists node'. auto.
-	}
-	wp_apply (newlock_spec with "Hhead_prop").
-	iIntros (hlock γh) "Hγh".
-	wp_let.
-	wp_apply (newlock_spec with "Htail_prop").
-	iIntros (tlock γt) "Hγt".
-	wp_let.
-	wp_alloc queue as "Hqueue".
-	iApply "HΦ".
-	iExists head, tail, hlock, tlock, γh, γt, queue.
-	iSplitR.
-	{ done. }
-	iFrame.
-	done.
+	wp_alloc l_queue as "Hl_queue".
+	iMod (pointsto_persist with "Hl_queue") as "#Hl_queue".
+	iApply ("HΦ" $! #l_queue Queue_gnames).
+	iModIntro.
+	iExists l_head, l_tail, hlock, tlock, l_queue.
+	auto.
 Qed.
 
-Lemma enqueue_spec Q (v : val) : {{{ is_queue Q }}}
-							 enqueue Q v 
-						 {{{w, RET w; True}}}.
+Lemma enqueue_spec Q (v : val) (qg : Qgnames) :
+	{{{ is_queue Q qg }}}
+		enqueue Q v 
+	{{{w, RET w; True}}}.
 Proof.
-	iIntros (Φ) "(%head & %tail & %H_lock & %T_lock & %γh & %γt & 
-				  %l & -> & Hq & #H_hlock & #H_tlock) HΦ".
+	iIntros (Φ) "(%l_head & %l_tail & %H_lock & %T_lock & %l_queue & -> &
+				 #Hl_queue & #H_queue_inv & #H_hlock & #H_tlock) HΦ".
 	wp_lam.
 	wp_let.
 	wp_pures.
-	wp_alloc null' as "Hnull'".
-	iMod (pointsto_persist with "Hnull'") as "#Hnull'".
-	wp_alloc null as "Hnull".
-	wp_alloc node' as "Hnode'".
-	iMod (pointsto_persist with "Hnode'") as "#Hnode'".
+	wp_alloc lₙ₂ as "Hlₙ₂".
+	wp_alloc l'ₙ₁ as "Hl'ₙ₁".
+	iMod (pointsto_persist with "Hl'ₙ₁") as "#Hl'ₙ₁".
 	wp_let.
 	wp_load.
 	wp_pures.
 	wp_apply (acquire_spec with "H_tlock").
-	iIntros "(Hlocked_γt & %tail' & Htail & Htail_inv)".
+	iIntros "(Hlocked_γ_Tlock & HTokE)".
 	wp_seq.
 	wp_load.
 	wp_pures.
-	wp_bind (! #tail)%E.
-	iInv "Htail_inv" as "(%x & %xs & H)". simpl in *.
-	iDestruct "H" as "(%tail_next & #Htail' & %tail_next' & Htail_next & Htail_next_inv)".
+	wp_bind (! #l_tail)%E.
+	iInv "H_queue_inv" as "(%xs & %xs_rest & %xs_old & %x_head & %x_tail & #Hxs_eq & HisLL_xs & >Hcases)".
+	iDestruct "Hcases" as "[HStatic | H]".
+	- (* Open in Static*)
+	iDestruct "HStatic" as "(Hl_head & [Hl_tail1 Hl_tail2] & [%xs_fromtail %H_isLast] & HToknE & HToknD & HTokUpdated)".
 	wp_load.
-	iSplitL "Htail_next Htail_next_inv".
+	iModIntro.
+	iAssert (fst x_tail ↦□ (snd x_tail, #(trd x_tail)) ∗ isLL (xs))%I with "[HisLL_xs]" as "[#Hx_tail HisLL_xs]".
+	{ 
+		rewrite H_isLast. iDestruct "HisLL_xs" as "[Hnull Hchain]".
+		destruct xs_fromtail.
+		- iPoseProof "Hchain" as "#Hchain". iFrame. auto.
+		- iDestruct "Hchain" as "[#H1 H2]"; iFrame. auto.
+	}
+	iDestruct "HTokUpdated" as "[HTokBefore HTokAfter]".
+	iPoseProof (isLL_and_chain with "HisLL_xs") as "[HisLL_xs #HisLL_chain_xs]".
+	iSplitL "Hl_head Hl_tail1 HTokE HToknD HTokBefore HisLL_xs".
+	(* Close in Enqueue: Before *)
 	{  
-		iExists x, xs, tail_next. iModIntro. iNext. iSplitR; first done.
-		iExists tail_next'. iSplitL "Htail_next"; done.
+		iNext. iExists xs, xs_rest, xs_old, x_head, x_tail.
+		iSplitR; first done.
+		iSplitL "HisLL_xs"; first done.
+		iRight. iLeft. 
+		iFrame. iLeft. iFrame. iPureIntro. exists xs_fromtail. done.
 	}
-	iModIntro.
-	wp_load.
-	wp_lam.
-	wp_match.
-	wp_pures.
-	wp_bind (#tail_next <- #node')%E.
-	(* STUCK: Don't know that tail_next points to something. *)
-	iInv "Htail_next_inv" as "(%l' & Htail_next & #Hl')".
-	wp_store.
-	iModIntro.
-	iSplitL "Htail_next".
-	{ iNext. iExists node. iFrame. }
-	wp_seq.
 	wp_load.
 	wp_pures.
-	wp_bind (#tail <- #node)%E.
-	iInv "Hinv" as "(%tl2 & Htail & Htl2node)".
-	wp_store.
-	iSplitL "Htail Hnode Hnext Hnull".
+	wp_bind (#(trd x_tail) <- #l'ₙ₁)%E.
+	iInv "H_queue_inv" as "(%xs_2 & %xs_rest_2 & %xs_old_2 & %x_head_2 & %x_tail_2 & #Hxs_eq_2 & HisLL_xs_2 & >Hcases_2)".
+	iDestruct "Hcases_2" as "[HStatic | H]".
+	+ (* Imossible: ToknE *) admit.
+	+ (* Open in Enqueue: Before *)
+	iDestruct "H" as "[HEnqueue | H]".
+	* 
+	iDestruct "HEnqueue" as "(Hl_head & Hl_tail1 & [([%xs_fromtail_2 %H_isLast_2] & HTokBefore) | (_ & HTokAfter2)] & HTokE & HToknD)".
+	**
+	iCombine "Hl_tail1 Hl_tail2" as "Hl_tail" gives "[_ %Htail_eq]".
+	iAssert (▷(trd x_tail ↦ NONEV ∗ isLL_chain xs_2))%I with "[HisLL_xs_2]" as "[Hnull HisLL_chain_xs_2]".
 	{
-		iMod (inv_alloc N _ (points_to_node next) with "[Hnext Hnull]") as "#Hnext".
+		iNext.
+		iAssert (fst x_tail_2 ↦□ (snd x_tail_2, #(trd x_tail_2)) ∗ isLL (xs_2))%I with "[HisLL_xs_2]" as "[#Hx_tail_2 HisLL_xs_2]".
 		{
-			iNext. iExists null. eauto.
+			rewrite H_isLast_2. iDestruct "HisLL_xs_2" as "[Hnull Hchain]".
+			destruct xs_fromtail_2.
+			- iPoseProof "Hchain" as "#Hchain". iFrame. auto.
+			- iDestruct "Hchain" as "[#H1 H2]"; iFrame. auto.
 		}
-		iModIntro. iNext. iExists node. iFrame. iExists next, (SOMEV v).
-		iSplitR. done. done.
+		iAssert (⌜x_tail = x_tail_2⌝%I) as "<-".
+		{ iApply fst_equal; auto. }
+		by rewrite H_isLast_2.
 	}
+	wp_store.
+	iAssert (fst x_tail_2 ↦□ (snd x_tail_2, #(trd x_tail_2)) ∗ isLL_chain xs_2)%I with "[HisLL_chain_xs_2]" as "[#Hx_tail_2 HisLL_chain_xs_2]".
+	{
+		rewrite H_isLast_2. destruct xs_fromtail_2.
+		- iPoseProof "HisLL_chain_xs_2" as "#HisLL_chain_xs_2". iFrame. auto.
+		- iDestruct "HisLL_chain_xs_2" as "[#H1 H2]"; iFrame. auto.
+	}
+	iAssert (⌜x_tail = x_tail_2⌝%I) as "<-".
+	{ iApply fst_equal; auto. }
+	iMod (pointsto_persist with "Hnull") as "#Hnull".
+	iDestruct "Hl_tail" as "[Hl_tail1 Hl_tail2]".
 	iModIntro.
+	set x_new := (l'ₙ₁, SOMEV v, lₙ₂).
+	set xs_new := x_new :: xs_2.
+	iAssert (isLL xs_new) with "[Hlₙ₂ HisLL_chain_xs_2]" as "HisLL_xs_new".
+	{
+		unfold xs_new, isLL. iFrame. rewrite H_isLast_2. iFrame. auto.
+	}
+	iPoseProof (isLL_and_chain with "HisLL_xs_new") as "[HisLL_xs_new #HisLL_chain_xs_new]".
+	iSplitL "Hl_head Hl_tail1 HTokE HToknD HTokAfter HisLL_xs_new".
+	(* Close in Enqueue: After *)
+	{
+		iNext. iExists xs_new, (x_new :: xs_rest_2), xs_old_2, x_head_2, x_tail.
+		iPoseProof "Hxs_eq_2" as "%Hxs_eq_2".
+		iSplitR. { iPureIntro. unfold xs_new. cbn. rewrite Hxs_eq_2. auto. }
+		iFrame.
+		iRight. iLeft.
+		iFrame. iRight. iFrame. iPureIntro. exists x_new, xs_fromtail_2.
+		unfold xs_new. by rewrite H_isLast_2.
+	}
 	wp_seq.
 	wp_load.
 	wp_pures.
-	wp_apply (release_spec with "[$H_tlock $Hlocked_γt $Hinv]").
-	iApply "HΦ".
+	wp_bind (#l_tail <- #l'ₙ₁)%E.
+	iInv "H_queue_inv" as "(%xs_3 & %xs_rest_3 & %xs_old_3 & %x_head_3 & %x_tail_3 & #Hxs_eq_3 & HisLL_xs_3 & >Hcases_3)".
+	iDestruct "Hcases_3" as "[HStatic | H]".
+	*** (* Imossible: ToknE *) admit.
+	*** (* Open in Enqueue: After *)
+	iDestruct "H" as "[HEnqueue | H]".
+	****
+	iDestruct "HEnqueue" as "(Hl_head & Hl_tail1 & [([%xs_fromtail_3 %H_isLast_3] & HTokBefore2) | ((%x_new_2 & %xs_fromtail_3 & %H_isSndLast) & HTokAfter)] & HTokE & HToknD)".
+	***** (* Impossible: TokBefore *) admit.
+	*****
+	iCombine "Hl_tail1 Hl_tail2" as "Hl_tail" gives "[_ %Htail_eq2]".
+	rewrite dfrac_op_own.
+	rewrite Qp.half_half.
+	wp_store.
+	iModIntro.
+	iAssert (isLL xs_3 ∗ isLL_chain xs_3)%I with "[HisLL_xs_3]" as "[HisLL_xs_3 #HisLL_chain_xs_3]".
+	{ by iApply isLL_and_chain. }
+	iAssert (⌜x_tail_3 = x_tail⌝)%I as "%Heq_x_tail".
+	{
+		iApply (isLL_chain_agree x_tail_3 x_tail [x_new_2] []).
+		- by simplify_eq.
+		- subst. iPoseProof (isLL_chain_split [x_new_2 ; x_tail_3] xs_fromtail_3 with "HisLL_chain_xs_3") as "[Hgoal _]". done.
+		- subst. iPoseProof (isLL_chain_split [x_tail] xs_fromtail with 
+		"HisLL_chain_xs") as "[Hgoal _]". done.
+	}
+	iAssert (⌜x_new_2 = x_new⌝)%I as "%Heq_x_new".
+	{
+		iApply (isLL_chain_agree_next x_tail x_new_2 x_new [] []).
+		- subst. iPoseProof (isLL_chain_split [x_new_2; x_tail] xs_fromtail_3 with "HisLL_chain_xs_3") as "[Hgoal _]". done.
+		- subst. iPoseProof (isLL_chain_split [x_new; x_tail] xs_fromtail_2 with "HisLL_chain_xs_new") as "[Hgoal _]". done.
+	}
+	iSplitR "HTokE Hlocked_γ_Tlock HΦ".
+	(* Close in Static *)
+	{
+		iNext. iExists xs_3, xs_rest_3, xs_old_3, x_head_3, x_new.
+		iSplitR; first done.
+		iFrame.
+		iLeft.
+		iFrame.
+		iPureIntro.
+		exists (x_tail_3 :: xs_fromtail_3).
+		subst. 
+		done.
+	}
+	wp_seq.
+	wp_load.
+	wp_pures.
+	wp_apply (release_spec with "[$H_tlock $HTokE $Hlocked_γ_Tlock]").
+	done.
 Qed.
 
 Lemma dequeue_spec Q : {{{ is_queue Q }}} 
